---
title: "Tao Analysis Solutions"
author: "Segun"
date: "21 de febrero de 2019"
output:
  pdf_document: default
  html_document: default
---

```{r setup, include=FALSE}
knitr::opts_chunk$set(echo = TRUE)
```



**Pg 24** Prove that the sum of two natural numbers is again a natural number?


*Solution*: Let $n$ and $m$ be natural numbers. Using induction on $n$ and keeping $m$ fixed,we have the base case to be $0 + m := m$ which is a natural number as desired (by definition of addition and **Axiom 2.1**). 

Now we assume inductively $n+m$ is a natural number. We have to show that $(n++)+m$ is also a natural number. But $(n++) + m = (n+m)++$ by definition of addition and **Axiom 2.2**. However, $n+m$ is a natural number according to the inductive hypothesis and therefore $(n+m)++$ is also a natural number by **Axiom 2.2**.
$\square$

**Pg 26** Prove that $n++ = n+1$ 

*Solution 1*: Let $n$ be a natural number, then $n++ = (n++) + 0 = (n+0)++ = n + (0++) = n+1$ according to **Lemma 2.2.2**, definition of addition, **Lemma 2.2.3** and definition of increment respectively. $\square$

*Solution 2*: Using induction on $n$, we have to show that $0++ = 0+1$ for the base case. However, $0++ = 1 = 0 + 1$ by definitions of increment, and addition respectively and so the base case is done. 

Now suppose inductively that $n++ = n+1$, we have to show that $(n++) ++ = (n++) +1$.

From the RHS, $(n++)+1 = (n+1)++ = (n++)++$ by definition of addition and the inductive hypothesis repectively. $\square$

**Exercise 2.2.1.** (Addition is associative). Prove that for any natural numbers $a$, $b$, $c$, we have $(a + b) + c = a + (b + c)$.

*Solution*: Using induction on $a$ and keeping $a$ and $c$ fixed. For the base case, we want to show that $(0+b) + c = 0+(b+c)$. However, $(0+b) + c  = b+c = 0 + (b+c)$ by the definition of addition.

Now suppose inductively that $(a+b)+c = a+(b+c)$, we have to show that $((a++)+b)+c = (a++) + (b+c)$.

From the RHS, we have that $(a++) + (b+c) = (a+(b+c))++ = ((a+b)+c)++$ by the definition of addition and the inductive hypothesis respectively. Furthermore, $((a+b)+c)++ = (((a+b)++)+c) = ((a++)+b)+c$ by definition of addition. $\square$

**Exercise 2.2.2.** Let $a$ be a positive number. Then there exists exactly one natural number $b$ such that $b++ = a$.

*Solution:* First we prove the existence of a natural number $b$ such that $b{++} = a$ for $a\in \mathbb{N}^+$ using induction on $a$. For the base case $a = 1$, we want to show that there exists a natural number $b$ such that $b{++} = 1$. Clearly, $0{++} = 1$ so $b = 0$.

Now suppose inductively that for any positive number $a$, there exists a natural number $b$ such that $b{++} = a$. 

We have to show that there exists a natural number $q$ such that $q++ = a++$. But $a++ = (b++)++$ by the inductive hypothesis, so that $q{++} = (b{++}){++}$ and by **Axiom 2.4**, $q = b{++}$. So that completes the induction and the proof existence.

Now we have to prove the uniqueness of the natural number $b$ such that $b{++} = a$ for $a\in \mathbb{N}^+$. Suppose for the sake of contradiction that there exist $b$, $c$ $\in \mathbb{N}$ with $b\ne c$ such that $b{++} = a$ and $c{++} = a$. Then $b{++} = c{++}$ and by **Axiom 2.4** $b = c$ which is a contradiction. Consequently, there exists exactly one natural number $b$ such that $b{++} = a$  for $a\in \mathbb{N}^+$. $\square$

**Exercise 2.2.3.** Basic properties of order for natural numbers). Let a, b, c be natural numbers. Then
*Solution:*
\begin{enumerate}
\item (Order is reflexive) $a \ge a$.

$a = a + 0$ by \textbf{Lemma 2.2.3} , therefore, $a\ge a$ by definition. $\square$

\item (Order is transitive) If $a \ge b$ and $b \ge c$, then $a \ge c$.

By definition, $a\ge b$ implies that $a = b+d$ and $b \ge c$ implies $b = c + e$, for some $d$, $e$ $\in \mathbb{N}$. Therefore, $a = b + d = (c+e)+d = c +(e+d) \ge c$ by ordering of natural numbers and associativity of addition. $\square$.   

\item (Order is anti-symmetric) If $a \ge b$ and $b \ge a$, then $a = b$.


Since $a \ge b$ and $b \ge a$, we have that $a = b + c$ and $b = a + d$ for some $c$, $d$ $\in \mathbb{N}$. Thus $a = a + c + d$ which implies that $c+d = 0$ by \textbf{Lemma 2.2.2} and that further implies $c = 0$ and $d = 0$ by \textbf{Corollary 2.2.9}. Consequently, $a = b$. $\square$


\item (Addition preserves order) $a \ge b$ if and only if $a + c \ge b + c$.

Because $a\ge b$, $a = b+d$ for some $d \in \mathbb{N}$. Hence $a + c = (b+d) + c = (b+c) + d \ge b+c$ by the cancellation law, associativity of addition and ordering of natural numbers respectively.

Likewise, $a+c \ge b+c$ implies $a+c = (b+c) + e$, for some $e \in \mathbb{N}$. Consequently, $a+c = (b+e) + c$ by associativity of addition. By cancellation law, $a = b + e$ so $a\ge b$. $\square$ 

\item $a < b$ if and only if $a{++} \le b$

\textit{Proof.} Since $a<b$,  then $b = a+n$, for some $n \in \mathbb{N}$ and $b \ne a$. Consequently, $n \ne 0$ by \textbf{Lemma 2.2.2}. Then there exists a number say $m \in \mathbb{N}$ such that $m{++} = n$ by \textbf{Lemma 2.2.10}. So $b = a+n = a + m{++} = (a{++}) + m$ by \textbf{Lemma 2.2.3}. So $a{++} \le b$.

Likewise $a{++} \le b$ implies $b = (a{++}) + n$ for some $n \in \mathbb{N}$. Consequently, $b = a + (n{++})$ by \textbf{Lemma 2.2.3} and by \textbf{Definition 2.2.1} (Addition of natural numbers). But we know that $n{++} \ne 0$ by \textbf{Axiom 2.3} and by implication $b \ne a$. So $a<b$. $\square$

\item $a < b$ if and only if $b = a + d$ for some positive number $d$.

\textit{Proof}. If $a<b$, then $b = a+d$ for some $d\in \mathbb{N}$ and $b\ne a$ by definition. We need to show that $d\ne 0$. Now suppose for the sake of contradiction that $d = 0$. Then $b = a+d$ implies $a = b$ which is a contradition so $d\ne0$. 

Likewise, $b = a+d$, $d \ne 0$ implies $a\le b$ by \textbf{Definition 2.2.11} (Ordering of the natural numbers). We need to show that $b \ne a$. Suppose for the sake of contradiction that $b = a$, then $b = a+d$ implies  $d = 0$ by \textbf{Lemma 2.2.2} which is a contradiction. Hence $b \ne a$ and $a\le b$ so $a<b$. $\square$

\end{enumerate}

**Exercise 2.2.4.** Justify the three statements marked (why?) in the proof of **Proposition 2.2.13**.

\begin{enumerate}
\item $0\le b$ for all $b\in \mathbb{N}$.

\textit{Proof}. Since $b \in \mathbb{N}$, then $b = 0 + b$ by \textbf{Definition 2.2.1} (Addition of natural numbers) so $0\le b$ by \textbf{Definition 2.2.11} (Ordering of the natural numbers). 

\item  If $a>b$, then $a{++} > b$

\textit{Proof}. Because $a{++}>a$ and $a>b$. Then by \textbf{Proposition 2.2.12} (Transitivity of order), $a{++} > b$. 

\item If $a = b$, the $a{++} =  b+d$

\textit{Proof}. Because $a{++}>a$ implies $a{++}>b$  since $a=b$. 

\end{enumerate}

**Exercise 2.2.5.** Prove **Proposition 2.2.14**. (Strong principle of induction). Let $m_0$ be a natural number, and let $P(m)$ be a property pertaining to an arbitrary natural number $m$. Suppose that for each $m \ge m_0$, we have the following implication: if $P(m')$ is true for all natural numbers $m_0 \le m' < m$ , then $P(m)$ is also true. (In particular, this means that $P(m_0)$ is true, since in this case the hypothesis is vacuous.) Then we can conclude that $P(m)$ is true for all natural numbers $m \ge m0$.

*Proof 1:* (Informal) Let $Q(n)$ be the property that $P(m)$ is true for all $m_o \le m < n$. Then if $n\le m_0$, then $Q(n)$ is vacuously true. If $n = m_0{++}$, then $Q(m_0{++})$ is true because $P(m)$ is true for all natural numbers $m_0 \le m < m_0{++}$ (since $P(m_0)$ is vacuously true) and by definition of $P$, $P(m_0{++})$ is also true. Likewise, if $n = (m_0{++})++$, then $Q((m_0{++})++)$ is true becuase  $P(m)$ is true for all $m_0 \le m < (m_0{++})++$ (since $P(m_0)$ and $P(m_0{++})$ are true) and by definition of $P$, $P((m_0{++})++)$ is also true. And so it goes on and on.    


*Proof:* Let $n\in \mathbb{N}$ and let $Q(n)$ be the property that $P(m)$ is true for all $m_0 \le m < n$ for $n\ge m_0$. Using induction on $n$, for the base case $n = 0$, we want to show that $Q(0)$ is true. However, we know that $0\le m_0\ \forall\ m_0 \in \mathbb{N}$. Thus, either $0 = m_0$ or $0<m_0$ and so we split into cases. If $n = 0 < m_0$, the statement $P(m)\ \forall\ m_0\le m < n$ is vacuously true (since the hypothesis applies for $n \ge m_0$) and thus $Q(0)$ is true in this case.  For the second case, if $n = 0 =m_0$, then the statement $P(m)\ \forall\ m_0\le m < n$ is also vacuously true since there is no $m' \in \mathbb{N}$ such that $0 \le m' <0$. Hence, $Q(0)$ is true for this case and that completes the base case of the induction. 

Now suppose inductively that for some $n\ge m_0$, $Q(n)$ is true, i.e $P(m)\ \forall\ m_0\le m < n$ is true. We need to show that $Q(n{++})$ is true. 

By the definition of $P$ in the hypothesis, $P(n)$ is also true (because $Q(n)$ is true). Since $n<n++$, then $P(m)\ \forall\ m_0\le m \le n < n++$ is true so $P(m)\ \forall\ m_0\le m < n++$ is true which in turn implies that $Q(n{++})$ is true. Which closes the induction and hence we can conclude that $Q(n)\ \forall n$ is true. 

However, $Q(n)$ true implies $P(m)\ \forall\ m_0\le m<n$ is true for all $n\ge m_0$ and by the definition of $P$, $P(n)$ is true  for all $n\ge m_0$ which concludes the proof. $\square$   



**Exercise 2.2.6.** Let $n$ be a natural number, and let $P(m)$ be a property pertaining to the natural numbers such that whenever $P(m{++})$ is true, then $P(m)$
is true. Suppose that $P(n)$ is also true. Prove that $P(m)$ is true for all natural
numbers $m \le n$; this is known as the principle of *backwards induction*. (Hint:
apply induction to the variable $n$.)


*Proof:* Let $n \in \mathbb{N}$. Using induction on $n$, for the base case $n = 0$, we need to show that $P(m)$ is true $\forall\ m\le 0$. But only $0\le 0$ so we just need to show that $P(0)$ is true. Since $P(n)$ is true from the hypothesis, $P(0)$ is true and that completes the base case. 

Suppose inductively that the principle if true for $n$, i.e $P$ is such that $P(n)$ is true, and whenever $P(m{++})$ is true, $P(m)$ is true $\forall m\le n$. We have to show the principle is true for $n{++}$ i.e we need to show that $P(m)$ is true $\forall\ m\le n++$ given that $P(n{++})$ is true and given that whenever $P(m{++})$ is true, $P(m)$ is true.

Since $P(n{++})$ is true, then $P(n)$ is also true. So we have to show that $P(m)$ is true $m<n$. But from the inductive hypothesis, $P(m)$ is true $\forall$ $m\le n$ and that completes the inductive hypothesis. $\square$


**Exercise 2.3.1.** Prove Lemma 2.3.2. (Multiplication is commutative). Let $n$, $m$ be natural numbers. Then $n \times m$ = $m \times n$. 

**Exercise 2.3.2.** Prove Lemma 2.3.3. (Positive natural numbers have no zero divisors). Let $n$, $m$ be natural numbers. Then $n \times m = 0$ if and only if at least one of $n$, $m$ is equal to zero. In particular, if $n$ and $m$ are both positive, then $nm$ is also positive.

**Exercise 2.3.3.** Prove Proposition 2.3.5. (Multiplication is associative). For any natural numbers $a$, $b$, $c$, we have $(a \times b) \times c = a \times (b \times c)$.

**Exercise 2.3.4.** Prove the identity $(a + b)^2 = a^2 + 2ab + b^2$ for all natural numbers $a$, $b$.

**Exercise 2.3.5.** Prove Proposition 2.3.9. (Euclidean algorithm). Let $n$ be a natural number, and let $q$ be a positive number. Then there exist natural numbers $m$, $r$ such that $0 \le r < q$ and $n = mq + r$. (*Hint*: fix $q$ and induct on $n$.)
